[WIP] teach poly ir that the exec_loop is also a function

backend/PolyIR.v
@@ -44,27 +44,28 @@ End EVAL_AFFINEEXPR.
 Section EXEC_STMT.
 Variable l: loop.
   
-  Inductive exec_stmt: lenv -> mem -> stmt -> mem -> lenv -> Prop :=
+  Inductive exec_stmt: lenv -> mem -> stmt -> mem -> Prop :=
   | exec_Sstore: forall (le: lenv) (m m': mem)
                    (chunk: memory_chunk) (addr: affineexpr) (i: int) (vaddr: val),
       eval_affineexpr le l addr vaddr ->
       Mem.storev chunk m vaddr (Vint i) = Some m' ->
-      exec_stmt le m (Sstore chunk addr i) m' le.
+      exec_stmt le m (Sstore chunk addr i) m'.
 End EXEC_STMT.
 
 Section EXEC_LOOP.
 
   Inductive exec_loop: lenv -> mem -> loop -> mem -> lenv -> Prop :=
   | eval_loop_stop: forall le m l,
-      (loopschedule l (viv le) >= (loopub l))%nat ->
+      (viv le >= loopub l)%nat ->
       exec_loop le m l m le
-  | eval_loop_loop: forall le le' le'' m m' m'' l,
-      exec_stmt l le m (loopstmt l) m' le' ->
-      exec_loop (lenv_bump_vindvar le) m' l m'' le'' ->
-      exec_loop le m l m'' le''.
+  | eval_loop_loop: forall le le' m m' m'' l,
+      (viv le < loopub l)%nat ->
+      exec_stmt l le m (loopstmt l) m' ->
+      exec_loop (lenv_bump_vindvar le) m' l m'' le' ->
+      exec_loop le m l m'' le'.
 End EXEC_LOOP.
 
-Theorem eval_affinexpr_is_function:
+Theorem eval_affineexpr_is_function:
   forall (le: lenv) (l: loop) (ae: affineexpr) (v v': val),
     eval_affineexpr le l ae v ->
     eval_affineexpr le l ae v' ->
@@ -75,6 +76,46 @@ Proof.
   intros eval_v'.
   induction ae; inversion eval_v; inversion eval_v'; subst; try auto.
 Qed.
+
+
+Theorem exec_stmt_is_function:
+  forall (le: lenv) (l: loop) (m m' m'': mem) (s: stmt),
+    exec_stmt l le m s m' ->
+    exec_stmt l le m s m'' ->
+    m' = m''.
+Proof.
+  intros until s.
+  intros eval_m.
+  intros eval_m'.
+  induction s; inversion eval_m;inversion eval_m'; subst; try auto.
+  assert(vaddr = vaddr0) as veq.
+  eapply eval_affineexpr_is_function; eassumption.
+  subst.
+  assert (Some m' = Some m'') as meq.
+  rewrite <- H14. rewrite <- H6.
+  reflexivity.
+  inversion meq. subst.
+  auto.
+Qed.
+
+Theorem exec_loop_is_function:
+  forall (le' le'': lenv) (viv: vindvar) (l: loop) (m m' m'': mem),
+    exec_loop (mkLenv viv) m l m' le' ->
+    exec_loop (mkLenv viv) m l m'' le'' ->
+    m' = m'' /\ le' = le''.
+Proof.
+  intros until m''.
+  intros exec_l1 exec_l2.
+  induction exec_l1; induction exec_l2; subst.
+  - auto.
+  - omega.
+  - omega.
+  -  assert (m' = m'0) as meq.
+     eapply exec_stmt_is_function; eassumption.
+     subst.
+     eapply IHexec_l1.
+     eassumption.
+Qed.
       
       
       
@@ -82,5 +123,4 @@ Qed.
     
     
   
-End EXEC_STMT.
   
